Concat

LTS.thy
@@ -22,9 +22,9 @@ a path. This leads to the following definition of reachability. Notice,
 that @{term "LTS_is_reachable \<Delta>"} is the reflexive, transitive closure of @{term \<Delta>}.\<close>
 
 inductive LTS_is_reachable :: "(('q, 'a) LTS * ('q * 'q) set) \<Rightarrow> 'q \<Rightarrow> 'a list \<Rightarrow> 'q \<Rightarrow> bool" where
-   LTS_Empty[intro!]:"LTS_is_reachable \<Delta> q [] q"|
-   LTS_Step1[intro!]:"(\<exists>q''. (q, q'') \<in> snd \<Delta> \<and> LTS_is_reachable \<Delta> q'' l q') \<Longrightarrow> LTS_is_reachable \<Delta> q l q'" |
-   LTS_Step2[intro!]:"(\<exists>q'' \<sigma>. a \<in> \<sigma> \<and> (q, \<sigma>, q'') \<in> fst \<Delta> \<and> LTS_is_reachable \<Delta> q'' w q') \<Longrightarrow> LTS_is_reachable \<Delta> q (a # w) q'"
+   LTS_Empty[intro!]:"LTS_is_reachable lts q [] q"|
+   LTS_Step1[intro!]:"(\<exists>q''. (q, q'') \<in> snd lts \<and> LTS_is_reachable lts q'' l q') \<Longrightarrow> LTS_is_reachable lts q l q'" |
+   LTS_Step2[intro!]:"(\<exists>q'' \<sigma>. a \<in> \<sigma> \<and> (q, \<sigma>, q'') \<in> fst lts \<and> LTS_is_reachable lts q'' w q') \<Longrightarrow> LTS_is_reachable lts q (a # w) q'"
 
 
 
@@ -35,33 +35,48 @@ inductive_cases LTS_Step2_cases:"LTS_is_reachable \<Delta> q l q'"
 inductive_cases LTS_Empty_cases:"LTS_is_reachable \<Delta> q [] q"
 
 
+lemma DeltLTSlemma1:"LTS_is_reachable l q al y \<Longrightarrow>LTS_is_reachable ({(f u a, v, f w a)| u v w. (u,v,w)\<in> fst l},{(f u a, f w a)| u w .(u,w) \<in> snd l}) (f q a) al (f y a)"
+  proof (induction rule: LTS_is_reachable.induct)
+    case (LTS_Empty lts q)
+    then show ?case by auto
+  next
+    case (LTS_Step1 q lts l q')
+    then show ?case apply auto
+      by blast
+  next
+    case (LTS_Step2 a q lts w q')
+    then show ?case apply auto by blast
+  qed
+
 
 lemma joinLTSlemma[simp]:"LTS_is_reachable l q x p \<Longrightarrow>  LTS_is_reachable l p y q''\<Longrightarrow> LTS_is_reachable l q (x@y) q''"
   proof (induction rule: LTS_is_reachable.induct)
-    case (LTS_Empty \<Delta> q)
-    then show ?case by auto
+    case (LTS_Empty lts q)
+    then show ?case apply auto done
   next
-    case (LTS_Step1 q \<Delta> l q')
-    then show ?case by auto
+    case (LTS_Step1 q lts l q')
+    then show ?case apply auto done
   next
-    case (LTS_Step2 a q \<Delta> w q')
-    then show ?case by auto
+    case (LTS_Step2 a q lts w q')
+    then show ?case apply auto done
   qed
+ 
+
+lemma notJoinLTSlemma:"\<forall>p. LTS_is_reachable l q x p \<and> \<not> LTS_is_reachable l p y q'' \<Longrightarrow> \<not> LTS_is_reachable l q (x@y) q''"
+  sorry
 
 lemma subLTSlemma[simp]:"LTS_is_reachable l1 q x y \<Longrightarrow> LTS_is_reachable (fst l1 \<union> l2, snd l1 \<union> l3) q x y"
   proof (induction rule: LTS_is_reachable.induct)
-    case (LTS_Empty \<Delta> q)
+    case (LTS_Empty lts q)
     then show ?case by auto
   next
-    case (LTS_Step1 q \<Delta> l q')
+    case (LTS_Step1 q lts l q')
     then show ?case by auto
   next
-    case (LTS_Step2 a q \<Delta> w q')
+    case (LTS_Step2 a q lts w q')
     then show ?case 
       by (smt (z3) LTS_is_reachable.LTS_Step2 UnI1 fst_conv)
   qed
-
-
 
 end
 (*
